rustfrontend/RustIRown.v
@@ -470,9 +470,7 @@ Inductive step_dropplace_mem_error: state -> Prop :=
 Inductive step : state -> trace -> state -> Prop :=
 | step_assign: forall f e p k le m1 m2 b ofs v v1 own1 own2 own3
     (* check ownership *)
-    (CHKEXPR: own_check_expr own1 e = true)
     (TFEXPR: move_place_option own1 (moved_place e) = own2)
-    (CHKASSIGN: own_check_assign own2 p = true)
     (TFASSIGN: own_transfer_assign own2 p = own3)
     (TYP: forall orgs id, typeof_place p <> Tvariant orgs id),
     (* get the location of the place *)
@@ -486,9 +484,7 @@ Inductive step : state -> trace -> state -> Prop :=
     step (State f (Sassign p e) k le own1 m1) E0 (State f Sskip k le own3 m2)
 | step_assign_variant: forall f e p ty k le m1 m2 m3 b ofs b1 ofs1 v v1 tag co fid enum_id orgs own1 own2 own3 fofs
     (* check ownership *)
-    (CHKEXPR: own_check_expr own1 e = true)
     (TFEXPR: move_place_option own1 (moved_place e) = own2)
-    (CHKASSIGN: own_check_assign own2 p = true)
     (TFASSIGN: own_transfer_assign own2 p = own3)
     (* necessary for clightgen simulation *)
     (TYP: typeof_place p = Tvariant orgs enum_id)
@@ -514,9 +510,7 @@ Inductive step : state -> trace -> state -> Prop :=
    step (State f (Sassign_variant p enum_id fid e) k le own1 m1) E0 (State f Sskip k le own3 m3)
 | step_box: forall f e p ty k le m1 m2 m3 m4 m5 b v v1 pb pofs own1 own2 own3
     (* check ownership *)
-    (CHKEXPR: own_check_expr own1 e = true)
     (TFEXPR: move_place_option own1 (moved_place e) = own2)
-    (CHKASSIGN: own_check_assign own2 p = true)
     (TFASSIGN: own_transfer_assign own2 p = own3),
     typeof_place p = Tbox ty ->
     (* Simulate malloc semantics to allocate the memory block *)
@@ -553,7 +547,6 @@ Inductive step : state -> trace -> state -> Prop :=
     step (State f (Sstoragedead id) k le own m) E0 (State f Sskip k le own m)
          
 | step_call: forall f a al k le m vargs tyargs vf fd cconv tyres p orgs org_rels own1 own2
-    (CHKEXPRLIST: own_check_exprlist own1 al = true)
     (TFEXPRLIST: move_place_list own1 (moved_place_list al) = own2), 
     classify_fun (typeof a) = fun_case_f tyargs tyres cconv ->
     eval_expr ge le m a vf ->
@@ -586,7 +579,6 @@ Inductive step : state -> trace -> state -> Prop :=
     (* return unit or Vundef? *)
     step (State f (Sreturn None) k e own m1) E0 (Returnstate Vundef (call_cont k) m2)
 | step_return_1: forall le a v v1 lb m1 m2 f k own1 own2
-    (CHKEXPR: own_check_expr own1 a = true)
     (TFEXPR: move_place_option own1 (moved_place a) = own2),
     eval_expr ge le m1 a v ->
     (* sem_cast to the return type *)
@@ -603,7 +595,6 @@ Inductive step : state -> trace -> state -> Prop :=
     step (State f Sskip k e own m1) E0 (Returnstate Vundef (call_cont k) m2)
 
 | step_returnstate: forall p v b ofs ty m1 m2 e f k own1 own2
-    (CHKASSIGN: own_check_assign own1 p = true)
     (TFASSIGN: own_transfer_assign own1 p = own2),
     eval_place ge e m1 p b ofs ->
     assign_loc ge ty m1 b ofs v m2 ->    
@@ -622,8 +613,7 @@ Inductive step : state -> trace -> state -> Prop :=
 | step_break_seq: forall f s k e m own,
     step (State f Sbreak (Kseq s k) e own m)
       E0 (State f Sbreak k e own m)
-| step_ifthenelse:  forall f a s1 s2 k e m v1 b ty own1
-    (CHKEXPR: own_check_expr own1 a = true),
+| step_ifthenelse:  forall f a s1 s2 k e m v1 b ty own1,
     (* there is no receiver for the moved place, so it must be None *)
     eval_expr ge e m a v1 ->
     to_ctype (typeof a) = ty ->
